LeanMove/Tests/Parsing/Test_extension_writes_after_join.lean
@@ -62,6 +62,6 @@ label l3:
   match parseAndTranslate extensionWritesAfterJoinMvir with
   | .ok results =>
     match findFun results "t" with
-    | some fd => alphaEquivFunDef fd t
+    | some fd => alphaEquivFunDef fd parsed_t
     | none => false
   | .error _ => false
